DynamoDbEncryption/dafny/DynamoDbEncryption/src/SearchInfo.dfy
@@ -17,15 +17,159 @@ module SearchableEncryptionInfo {
   import opened Wrappers
   import opened StandardLibrary.UInt
   import SortedSets
+  import Sets
+  import KeyStore = AwsCryptographyKeyStoreTypes
+  import Aws.Cryptography.Primitives
+  import Prim = AwsCryptographyPrimitivesTypes
 
   newtype VersionNumber = uint64
   type ValidSearchInfo = x : SearchInfo | x.ValidState?() witness *
+
+  class DumbCache {
+    var keyId : string
+    var keys : HmacKeyMap
+
+    constructor()
+    {
+      this.keyId := "";
+      this.keys := map[];
+    }
+
+    method get(s : string) returns (output : Option<HmacKeyMap>)
+    {
+      if keyId == s {
+        return Some(keys);
+      }
+      return None;
+    }
+    method put(s : string, k : HmacKeyMap)
+      modifies this
+    {
+      keyId := s;
+      keys := k;
+    }
+  }
+  type ValidStore = x : AwsCryptographyKeyStoreTypes.IKeyStoreClient | x.ValidState() witness *
+
+  datatype KeyLocation =
+    | LiteralKey (key: Bytes)
+    | SingleLoc (keyId: string)
+    | MultiLoc (keyName : string)
+
+  datatype KeySource = KeySource(
+    client : Primitives.AtomicPrimitivesClient,
+    cache : DumbCache,
+    store : ValidStore,
+    keyLoc : KeyLocation
+  ) {
+    function Modifies() : set<object> {
+      client.Modifies + store.Modifies + {cache}
+    }
+    predicate ValidState() {
+      client.ValidState() && store.ValidState()
+    }
+    method getKeyMap(beacons : BeaconMap) returns (output : Result<HmacKeyMap, Error>)
+      requires ValidState()
+      ensures ValidState()
+      modifies Modifies()
+    {
+      if keyLoc.SingleLoc? {
+        output := getKeys(beacons, keyLoc.keyId);
+      } else if keyLoc.LiteralKey? {
+        output := getAllKeys(beacons, "Literal", keyLoc.key);
+      } else {
+        output := Failure(E("Multi Tenant not yet implemented"));
+      }
+    }
+
+    method getKeys(beacons : BeaconMap, keyId : string) returns (output : Result<HmacKeyMap, Error>)
+      requires ValidState()
+      ensures ValidState()
+      modifies Modifies()
+    {
+      var k := cache.get(keyId);
+      if k.Some? {
+        return Success(k.value);
+      }
+      var key :- getKeyFromStore(keyId);
+      output := getAllKeys(beacons, keyId, key);
+    }
+
+    method getAllKeys(beacons : BeaconMap, keyId : string, key : Bytes) returns (output : Result<HmacKeyMap, Error>)
+      requires ValidState()
+      ensures ValidState()
+      modifies Modifies()
+    {
+      var beaconKeys := SortedSets.ComputeSetToOrderedSequence2(beacons.Keys, CharLess);
+      var stdKeys := Seq.Filter((k : string) => k in beacons && beacons[k].Standard?, beaconKeys);
+      var newKeys :- getHmacKeys(stdKeys, key, beacons);
+      cache.put(keyId, newKeys);
+      return Success(newKeys);
+    }
+
+    method {:tailrecursion} getHmacKeys(
+      beaconKeys : seq<string>,
+      key : Bytes,
+      beacons : BeaconMap,
+      acc : HmacKeyMap := map[]
+    )
+      returns (output : Result<HmacKeyMap, Error>)
+      requires forall k <- beaconKeys :: k in beacons
+      requires forall k <- acc :: k in beacons
+      ensures output.Success? ==> forall k <- output.value :: k in beacons
+
+      modifies client.Modifies
+      requires client.ValidState()
+      ensures client.ValidState()
+    {
+      if |beaconKeys| == 0 {
+        return Success(acc);
+      } else {
+        var key :- getBeaconKey(key, beaconKeys[0]);
+        output := getHmacKeys(beaconKeys[1..], key, beacons, acc[beaconKeys[0] := key]);
+      }
+    }
+
+    method getKeyFromStore(keyId : string)
+      returns (output : Result<Bytes, Error>)
+      modifies store.Modifies
+      requires store.ValidState()
+      ensures store.ValidState()
+    {
+      var maybeKey := store.GetBeaconKey(
+        KeyStore.GetBeaconKeyInput(
+          branchKeyIdentifier := keyId,
+          awsKmsKeyArn := None
+        )
+      );
+      var key :- maybeKey.MapFailure(e => AwsCryptographyKeyStore(e));
+      output := Success(key.beaconKey);
+    }
+
+    // convert persistent key to the derived key for this beacon
+    method getBeaconKey(key : Bytes, name : string)
+      returns (output : Result<Bytes, Error>)
+      modifies client.Modifies
+      requires client.ValidState()
+      ensures client.ValidState()
+    {
+      var info :- UTF8.Encode("AWS_DBE_SCAN_BEACON" + name).MapFailure(e => E(e));
+      var keyR := client.Hkdf(Prim.HkdfInput(
+        digestAlgorithm := Prim.SHA_512,
+        salt := None,
+        ikm := key,
+        info := info,
+        expectedLength := 64
+      ));
+      var key :- keyR.MapFailure(e => AwsCryptographyPrimitives(e));
+      return Success(key);
+    }
+  }
 
   datatype SearchInfo = SearchInfo(
     versions : seq<BeaconVersion>,
     currWrite : nat // index into `versions` for current version being written
   ) {
-
     function method CheckValid() : (ret : Result<bool, Error>)
       ensures ret.Success? ==> ValidState?()
     {
@@ -34,10 +178,18 @@ module SearchableEncryptionInfo {
       Success(true)
     }
 
+    function Modifies() : set<object>
+    {
+      set x, y | y in versions && x in y.Modifies() :: x
+    }
     predicate method ValidState?()
     {
       && 0 < |versions|
       && currWrite < |versions|
+      && forall v <- versions :: v.ValidState?()
+    }
+    predicate ValidState()
+    {
       && forall v <- versions :: v.ValidState()
     }
 
@@ -72,10 +224,13 @@ module SearchableEncryptionInfo {
       versions[currWrite].GenerateClosure(fields)
     }
 
-    function method GenerateBeacons(item : DDB.AttributeMap) : Result<DDB.AttributeMap, Error>
+    method GenerateBeacons(item : DDB.AttributeMap) returns (output : Result<DDB.AttributeMap, Error>)
       requires ValidState?()
+      requires ValidState()
+      ensures ValidState()
+      modifies Modifies()
     {
-      versions[currWrite].GenerateBeacons(item)
+      output := versions[currWrite].GenerateBeacons(item);
     }
   }
 
@@ -136,11 +291,12 @@ module SearchableEncryptionInfo {
       else
         cmp.GetFields(virtualFields)
     }
-    function method GetBeaconValue(value : DDB.AttributeValue, keys : HmacKeyMap, naked : bool) : Result<DDB.AttributeValue, Error>
+    function method GetBeaconValue(value : DDB.AttributeValue, keys : Option<HmacKeyMap>) : Result<DDB.AttributeValue, Error>
     {
-      if naked then
+      if keys.None? then
         Success(value)
       else
+        var keys := keys.value;
         if Standard? then
           if std.base.name in keys then
             std.GetBeaconValue(value, keys[std.base.name])
@@ -169,19 +325,27 @@ module SearchableEncryptionInfo {
 
   datatype BeaconVersion = BeaconVersion (
     version : VersionNumber,
+    keySource : KeySource,
     beacons : BeaconMap,
-    virtualFields : VirtualFieldMap,
-    hmacKeys : HmacKeyMap
+    virtualFields : VirtualFieldMap
   ) {
 
-    predicate method ValidState()
+    function Modifies() : set<object>
+    {
+      keySource.Modifies()
+    }
+
+    predicate method ValidState?()
     {
       && version == 1
       && (forall k <- virtualFields :: virtualFields[k].name == k)
       && (forall k <- beacons :: beacons[k].getName() == k)
       && (forall k <- virtualFields :: virtualFields[k].ValidState())
       && (forall k <- beacons :: beacons[k].ValidState())
-      && hmacKeys.Keys == beacons.Keys
+    }
+    predicate ValidState()
+    {
+      keySource.ValidState()
     }
 
     function method ValidStateResult() : Result<bool, Error>
@@ -216,10 +380,27 @@ module SearchableEncryptionInfo {
       SortedSets.ComputeSetToOrderedSequence2(fieldSet, CharLess)
     }
 
-    function method GenerateBeacons(item : DDB.AttributeMap, naked : bool := false) : Result<DDB.AttributeMap, Error>
+    method getKeyMap() returns (output : Result<HmacKeyMap, Error>)
+      requires ValidState()
+      ensures ValidState()
+      modifies Modifies()
+    {
+      output := keySource.getKeyMap(beacons);
+    }
+
+    method GenerateBeacons(item : DDB.AttributeMap, naked : bool := false)
+      returns (output : Result<DDB.AttributeMap, Error>)
+      requires ValidState()
+      ensures ValidState()
+      modifies Modifies()
     {
       var beaconNames := SortedSets.ComputeSetToOrderedSequence2(beacons.Keys, CharLess);
-      GenerateBeacons2(beaconNames, item, if naked then None else Some(hmacKeys))
+      if naked { 
+        output := GenerateBeacons2(beaconNames, item, None);
+      } else {
+        var hmacKeys :- getKeyMap();
+        output := GenerateBeacons2(beaconNames, item, Some(hmacKeys));
+      }
     }
 
     function method GenerateBeacon(name : string, item : DDB.AttributeMap, keys : Option<HmacKeyMap>) : Result<Option<DDB.AttributeValue>, Error>
